Euclidean Cross Product : 
 
a x b    = (a1e1 +a2e2+a3e3 ) x  (b1e1 + b2e2 + b3e3 ) =

= ( a1b2 -  a2b1 ) (e3) +  ( a3b1  - a1b3 ) (e2 )  +  ( a2b3 -  a3b2 ) ( e1  )  
 
Formula: 

\overrightarrow{a} \times  \overrightarrow{b} =\begin{bmatrix}e_{1}&e_{2}&e_{3}\\a_{1}&a_{2}&a_{3}\\b_{1}&b_{2}&b_{3}\end{bmatrix}

![det_Cross](https://github.com/probaxeoxebra/probaMinkoski/blob/master/FORMULAS/detCrossEucl.jpg)
 
………………………………………. 

http://www.sciweavers.org/free-online-latex-equation-editor

……………….
 
Minkowskian Cross Product:    

a x b    =  ( a1e1 +a2e2 +a0e0 )  x  (b1e1 + b2e2 +  b0e0  )  =  

=    ( a1b2 -  a2b1 ) (- e0 )  + ( a0b1 -  a1b0 )-e2) +  ( a2b0  - a0b2 ) ( e1)  
 
 
Formula:

\overrightarrow{a} \times  \overrightarrow{b} =\begin{bmatrix}e_{1}&e_{2}&-e_{0}\\a_{1}&a_{2}&a_{0}\\b_{1}&b_{2}&b_{0}\end{bmatrix}

![det_stCross](https://github.com/probaxeoxebra/probaMinkoski/blob/master/FORMULAS/detCrossMink.jpg)
